Implemented MPPC_natDeduct in new typeclasses

src/deduction/MPPC_natDeduct.lean
@@ -1,4 +1,7 @@
-import deduction.deduction data.set.basic
+import deduction.deduction_cartesian data.set.basic
+open deduction_basic
+
+
 
 namespace MPPC_defn
 
@@ -9,38 +12,32 @@ namespace MPPC_defn
     | impl : MPPC_Form → MPPC_Form → MPPC_Form
     | diamond : MPPC_Form → MPPC_Form
 
-
-    notation (name:=MPPC.top) `⊤`:80   := MPPC_Form.top
-    prefix `p`:80     := MPPC_Form.var
-    infix `&`:79      := MPPC_Form.and    
-    notation (name:= MPPC_Form.impl) φ `⊃`:80 ψ := MPPC_Form.impl φ ψ 
-    notation (name:= MPPC_Form.diamond) `◇`:max φ := MPPC_Form.diamond φ 
+    prefix `p`:80     := MPPC_Form.var  
+    notation (name:= MPPC_Form.diamond) `◇`:max φ := MPPC_Form.diamond φ
 
 
     @[reducible] def MPPC_Hyp : Type := set (MPPC_Form)
 
     instance : has_union MPPC_Hyp := infer_instance
-    instance : has_singleton MPPC_Form MPPC_Hyp := infer_instance
     instance : has_mem MPPC_Form MPPC_Hyp := infer_instance
     instance : has_insert MPPC_Form MPPC_Hyp := infer_instance
     instance : has_emptyc MPPC_Hyp := infer_instance
-    instance : is_lawful_singleton MPPC_Form MPPC_Hyp := infer_instance
 
     inductive MPPC_derives : MPPC_Hyp → MPPC_Form → Prop 
     | hyp {Φ : MPPC_Hyp} {φ : MPPC_Form}  
         : (φ ∈ Φ) →  MPPC_derives Φ φ
     | truth {Φ}                               
-        : MPPC_derives Φ ⊤ 
+        : MPPC_derives Φ MPPC_Form.top 
     | and_intro {Φ} {φ ψ : MPPC_Form}    
-        : MPPC_derives Φ φ → MPPC_derives Φ ψ → MPPC_derives Φ (φ & ψ)
+        : MPPC_derives Φ φ → MPPC_derives Φ ψ → MPPC_derives Φ (MPPC_Form.and φ ψ)
     | and_eliml {Φ} {φ ψ : MPPC_Form}    
-        : MPPC_derives Φ (φ & ψ) → MPPC_derives Φ φ
+        : MPPC_derives Φ (MPPC_Form.and φ ψ) → MPPC_derives Φ φ
     | and_elimr {Φ} {φ ψ : MPPC_Form}    
-        : MPPC_derives Φ (φ & ψ) → MPPC_derives Φ ψ
+        : MPPC_derives Φ (MPPC_Form.and φ ψ) → MPPC_derives Φ ψ
     | impl_intro {Φ : MPPC_Hyp} (φ : MPPC_Form) {ψ : MPPC_Form}   
-        : MPPC_derives (insert φ Φ) ψ → MPPC_derives Φ (φ ⊃ ψ)
+        : MPPC_derives (insert φ Φ) ψ → MPPC_derives Φ (MPPC_Form.impl φ ψ)
     | impl_elim {Φ : MPPC_Hyp} (φ : MPPC_Form) {ψ : MPPC_Form} 
-        : MPPC_derives Φ (φ ⊃ ψ) → MPPC_derives Φ φ → MPPC_derives Φ ψ
+        : MPPC_derives Φ (MPPC_Form.impl φ ψ) → MPPC_derives Φ φ → MPPC_derives Φ ψ
     | weak {Φ Ψ : MPPC_Hyp} {φ : MPPC_Form}
         : MPPC_derives Φ φ → MPPC_derives (Φ ∪ Ψ) φ
     | dmap {φ ψ : MPPC_Form}
@@ -55,181 +52,76 @@ namespace MPPC_defn
 end MPPC_defn
 
 
-
-
-
 namespace MPPC_has_derives
 
     open MPPC_defn
     open MPPC_defn.MPPC_derives
-    lemma internal1_impl : ∀ {φ ψ : MPPC_Form}, MPPC_derives {ψ} φ → MPPC_derives ∅ (ψ ⊃ φ) :=
+    open deduction_basic
+    open deduction_cart
+
+    instance MPPC_hasHyp : has_Hyp MPPC_Form :=
+      { Hyp := MPPC_Hyp }
+
+    instance MPPC_singleton : has_singleton MPPC_Form MPPC_Hyp :=
+      deduction_basic.singleHyp
+    @[simp] 
+    lemma same_singles : ∀ φ : MPPC_Form, 
+        MPPC_has_derives.MPPC_singleton.singleton φ = set.has_singleton.singleton φ :=
     begin 
-        assume φ ψ h,
-        apply impl_intro,
-        rw set.is_lawful_singleton.insert_emptyc_eq,
-        exact h,
-    end
-    lemma empty_union : ∀ φ : MPPC_Form, {φ} = ∅ ∪ MPPC_Hyp.has_singleton.singleton φ :=
-    begin
-        assume φ,
-        symmetry,
-        apply set.empty_union,
-    end
-    lemma weak1 : ∀ (φ ψ : MPPC_Form), MPPC_derives ∅ ψ → MPPC_derives {φ} ψ :=
-    begin 
-        assume φ ψ h,
-        rw empty_union,
-        apply weak,
-        exact h,
-    end
-    lemma MPPC_derive_refl : ∀ φ, MPPC_derives {φ} φ :=
-      λ φ, hyp (set.mem_singleton φ)
-
-    lemma MPPC_derive_trans : ∀ (φ ψ θ : MPPC_Form),
-        MPPC_derives {φ} ψ → MPPC_derives {ψ} θ → MPPC_derives {φ} θ :=
-    begin
-        assume φ ψ θ hφψ hψθ,
-        have helper : MPPC_derives {φ} (ψ ⊃ θ), 
-        apply weak1,
-        apply internal1_impl,
-        exact hψθ,
-        apply impl_elim,
-        exact helper,
-        exact hφψ,
+      assume φ,
+      dsimp[MPPC_has_derives.MPPC_singleton,deduction_basic.singleHyp],
+      rw set.is_lawful_singleton.insert_emptyc_eq,
     end
 
+    lemma single_union {Φ : MPPC_Hyp} {φ : MPPC_Form}
+        : insert φ Φ = {φ} ∪ Φ := by simp
 
-    instance MPPC_Der : has_derives MPPC_Form :=
-      ⟨   
-        MPPC_Hyp, 
-        MPPC_derives, 
-        MPPC_derive_refl, 
-        MPPC_derive_trans
-      ⟩ 
+
+    instance MPPC_Der : has_struct_derives MPPC_Form :=
+    {
+      derives := MPPC_derives,
+      derive_Trans := 
+        begin
+          assume Φ ψ θ hφψ hψθ,
+          have helper : MPPC_derives Φ (MPPC_Form.impl ψ θ),
+            apply impl_intro,
+            rw single_union,
+            apply weak,
+            exact hψθ,
+          apply impl_elim ψ,
+          exact helper,
+          exact hφψ,
+        end,
+      inInsert := set.mem_insert,
+      hyp := @hyp,
+      weak1 := 
+        begin
+          assume Φ φ ψ h,
+          rw single_union,
+          rw set.union_comm,
+          apply weak,
+          exact h,
+        end,
+    }
+
+    instance MPPC_top : deduction_cart.has_top MPPC_Form :=
+    {
+      top := MPPC_Form.top,
+      truth := @truth,
+    }
+    instance MPPC_and : deduction_cart.has_and MPPC_Form :=
+    {
+      and := MPPC_Form.and,
+      and_intro := @and_intro,
+      and_eliml := @and_eliml,
+      and_elimr := @and_elimr,
+
+    }
+    instance MPPC_impl : deduction_cart.has_impl MPPC_Form :=
+    {
+      impl := MPPC_Form.impl,
+      impl_intro := @impl_intro,
+      impl_elim := @impl_elim,
+    }
 
 end MPPC_has_derives
-
-
-
-namespace MPPC_Hyp_x
-
-    open MPPC_defn
-
-    @[simp] lemma lawful_singleton : ∀ {φ : MPPC_Form},
-        MPPC_Hyp.has_insert.insert φ MPPC_Hyp.has_emptyc.emptyc =
-        MPPC_Hyp.has_singleton.singleton φ := 
-        MPPC_defn.MPPC_Hyp.is_lawful_singleton.insert_emptyc_eq
-
-
-    meta def find_it : tactic unit :=
-        `[ repeat {{left,refl} <|> right}, try{apply set.mem_singleton}  ]
-
-    lemma insert_is_union_singleton : ∀ (Φ : MPPC_Hyp) (φ : MPPC_Form),
-        insert φ Φ = Φ ∪ {φ} :=
-        begin
-        assume Φ φ,
-        apply set.ext,
-        assume ψ,
-        apply or_comm,
-        end
-    lemma Hyp_twoElt_comm : ∀ (φ ψ : MPPC_Form), insert φ {ψ} = insert ψ (MPPC_Hyp.has_singleton.singleton φ) :=
-    begin
-        assume φ ψ,
-        apply set.ext,
-        assume θ,
-        apply or_comm,
-    end
-end MPPC_Hyp_x
-
-namespace MPPC_derives_x
-    open MPPC_defn
-    open MPPC_defn.MPPC_derives
-    open MPPC_has_derives
-    open MPPC_Hyp_x
-
-    lemma trans_hyp : ∀ (Φ : MPPC_Hyp) (φ ψ: MPPC_Form), MPPC_derives Φ φ → φ ⊢ ψ → MPPC_derives Φ ψ :=
-    begin 
-        assume Φ φ ψ hΦφ hφψ,
-        have helper : MPPC_derives Φ (φ ⊃ ψ),
-        apply impl_intro,
-        rewrite insert_is_union_singleton, 
-        rewrite set.union_comm,
-        apply weak,
-        exact hφψ,
-        apply impl_elim,
-        exact helper,
-        exact hΦφ,
-    end 
-
-    lemma modus_ponens : ∀ φ ψ : MPPC_Form, MPPC_derives ({φ⊃ψ,φ}) ψ :=
-    begin
-        assume φ ψ,
-        apply impl_elim,
-        apply weak,
-        apply MPPC_derive_refl,
-        rewrite Hyp_twoElt_comm,
-        apply weak,
-        apply MPPC_derive_refl,
-    end 
-
-    -- -- lemma hypo_syll : ∀ φ ψ θ, (φ ⊃ ψ) ⊢ ((ψ ⊃ θ) ⊃ (φ ⊃ θ)) := sorry
-
-    lemma hypo_syll' : ∀ φ ψ θ, (ψ ⊃ θ) ⊢ ((φ ⊃ ψ) ⊃ (φ ⊃ θ)) :=
-    begin 
-        assume φ ψ θ,
-        apply impl_intro,
-        apply impl_intro,
-        apply impl_elim ψ,
-        apply hyp, find_it,
-        apply impl_elim φ,
-        apply hyp, find_it,
-        apply hyp, find_it,
-    end 
-
-    lemma union_Hyp_and : ∀ φ ψ θ : MPPC_Form, MPPC_derives ({φ,ψ}) θ → ((φ&ψ) ⊢ θ) :=
-    begin 
-        assume φ ψ θ h,
-        apply impl_elim φ,
-        apply impl_elim ψ,
-        apply weak1,
-        apply impl_intro ψ,
-        rw set.is_lawful_singleton.insert_emptyc_eq,
-        apply impl_intro φ,
-        exact h,
-        apply and_elimr,
-        apply MPPC_derive_refl,
-        apply and_eliml,
-        apply MPPC_derive_refl,
-    end 
-
-    lemma and_Hyp_union : ∀ φ ψ θ : MPPC_Form, ((φ&ψ) ⊢ θ) → MPPC_derives ({ψ,φ}) θ :=
-    begin
-        assume φ ψ θ h,
-        apply impl_elim,
-        apply weak,
-        apply weak1,
-        apply internal1_impl,
-        exact h,
-        apply and_intro,
-        rw Hyp_twoElt_comm,
-        apply weak,
-        apply MPPC_derive_refl,
-        apply MPPC_derives.weak,
-        apply MPPC_derive_refl,
-    end 
-
-end MPPC_derives_x
-
-
--- open MPPC_defn
--- open MPPC_defn.MPPC_derives
--- open MPPC_has_derives
-
--- example : ∀ φ, MPPC_has_derives.MPPC_Der.derives ∅ (φ ⊃ ◇φ) :=
--- begin
---     assume φ,
---     apply impl_intro,
---     apply dpure,
---     simp[MPPC_Hyp_x.lawful_singleton],
---     exact (MPPC_derive_refl φ),
--- end
